better naming

Examples/OneTimePad.lean
@@ -17,32 +17,27 @@ open Mathlib OracleSpec OracleComp OracleAlg OracleImpl ENNReal BigOperators
 /-- The one-time pad symmetric encryption algorithm, using `BitVec`s as keys and messages.
 Encryption and decryption both just apply `BitVec.xor` with the key.
 Requires no oracles so the `OracleSpec` is always `[]ₒ`. -/
-def oneTimePad' (n : ℕ) : SymmEncAlg' []ₒ Unit
+def oneTimePad (n : ℕ) : SymmEncAlg []ₒ Unit
     (BitVec n) (BitVec n) (BitVec n) where
   keygen := $ᵗ BitVec n
   encrypt k m := return k ^^^ m
   decrypt k σ := return k ^^^ σ
   __ := emptyImpl
 
-/-- The one-time pad symmetric encryption algorithm, using `BitVec`s as keys and messages.
-Encryption and decryption both just apply `BitVec.xor` with the key.
-Requires no oracles so the `OracleSpec` is always `[]ₒ`. -/
-def oneTimePad : SymmEncAlg (λ _ ↦ []ₒ) BitVec BitVec BitVec where
-  keygen n := $ᵗ BitVec n
-  encrypt _ k m := return k ^^^ m
-  decrypt _ k σ := return k ^^^ σ
-  __ := baseOracleAlg
-
 namespace oneTimePad
 
 @[simp]
-lemma keygen_def (n : ℕ) : oneTimePad.keygen n = $ᵗ BitVec n := rfl
+lemma keygen_def (n : ℕ) : (oneTimePad n).keygen = $ᵗ BitVec n := rfl
 
 @[simp]
 lemma encrypt_bind_decrypt {n : ℕ} (k m : BitVec n) :
-    do {let σ ← oneTimePad.encrypt _ k m; oneTimePad.decrypt _ k σ} = return m := by
+    do {let σ ← (oneTimePad n).encrypt k m; (oneTimePad n).decrypt k σ} = return m := by
   simp [oneTimePad]
 
-theorem isSound : oneTimePad.isSound := λ sp m ↦ probOutput_eq_one (by simp)
+theorem isSound (n : ℕ) : (oneTimePad n).isSound :=
+  λ m ↦ probOutput_eq_one (by {
+    simp
+    sorry
+  })
 
 end oneTimePad
