VCVio/CryptoFoundations/SymmEncAlg.lean
@@ -14,58 +14,29 @@ for symmetric encryption using oracles in `spec`, with message space `M`,
 secret keys of type `K`, and ciphertext space `C`.
 -/
 
-open OracleSpec OracleComp OracleAlg BigOperators
+open OracleSpec OracleComp Prod
 
-structure SymmEncAlg' {ι : Type} (spec : OracleSpec ι) (σ M K C : Type)
+structure SymmEncAlg {ι : Type} (spec : OracleSpec ι) (σ M K C : Type)
     extends OracleImpl spec σ where
   keygen : OracleComp (unifSpec ++ₒ spec) K
   encrypt (k : K) (m : M) : OracleComp (unifSpec ++ₒ spec) C
   decrypt (k : K) (c : C) : OracleComp (unifSpec ++ₒ spec) M
 
-structure SymmEncAlg {ι : Type} (spec : ℕ → OracleSpec ι) (M K C : ℕ → Type)
-    extends OracleAlg spec where
-  (keygen (sp : ℕ) : OracleComp (unifSpec ++ₒ spec sp) (K sp))
-  (encrypt (sp : ℕ) : K sp → M sp → OracleComp (unifSpec ++ₒ spec sp) (C sp))
-  (decrypt (sp : ℕ) : K sp → C sp → OracleComp (unifSpec ++ₒ spec sp) (M sp))
-
 namespace SymmEncAlg
 
-variable {ι : Type} {spec : ℕ → OracleSpec ι} {M K C : ℕ → Type}
+variable {ι : Type} {spec : OracleSpec ι} {σ M K C : Type}
 
 section isSound
-
-variable [Π sp, DecidableEq (M sp)]
 
 /-- A symmetric encryption algorithm is sound is messages decrypt to themselves given a random key.
 Note that we assume the algorithm never fails, although in general this could be modified
 to allow for a (negligible) chance of encryption failure. -/
-def isSound (encAlg : SymmEncAlg spec M K C) : Prop :=
-  ∀ sp : ℕ, ∀ m : M sp, [= m | do
-    let k ← encAlg.keygen sp
-    let σ ← encAlg.encrypt sp k m
-    encAlg.decrypt sp k σ] = 1
-
-def isSound' {ι : Type} {spec : OracleSpec ι} {σ M K C : Type}
-    (encAlg : SymmEncAlg' spec σ M K C) : Prop :=
-  ∀ m : M, [= m | Prod.fst <$> (encAlg.exec do
+def isSound (encAlg : SymmEncAlg spec σ M K C) : Prop :=
+  ∀ m : M, [= m | fst <$> encAlg.exec do
     let k : K ← encAlg.keygen
     let σ ← encAlg.encrypt k m
-    encAlg.decrypt k σ)] = 1
-
-variable (encAlg : SymmEncAlg spec M K C)
-
--- lemma isSound_iff {ι : Type} {spec : OracleSpec ι} {M K C : Type}
---     (encAlg : SymmEncAlg' spec M K C) : encAlg.isSound ↔
---     ∀ m : M, ()
-
--- lemma isSound_iff_forall_mem_support :
+    encAlg.decrypt k σ] = 1
 
 end isSound
-
--- section perfectSecrecy
-
-
-
--- end perfectSecrecy
 
 end SymmEncAlg
