VCVio/OracleComp/OracleImpl.lean
@@ -26,20 +26,47 @@ a `ProbComp` that can be run with `OracleComp.runIO`.
 The types of primitives can extend this to ensure that any oracles used in a protocol
 must have some canonical implementation. -/
 structure OracleImpl {ι : Type} (spec : OracleSpec ι) (σ : Type) where
+  /-- Simulation oracle giving an implementation of the oracles in `spec`. -/
   baseSimOracle : spec →[σ]ₛₒ unifSpec
   init_state : σ
 
-def OracleImpl.exec {ι : Type} {spec : OracleSpec ι} {α σ : Type}
-    (impl : OracleImpl spec σ) (oa : OracleComp (unifSpec ++ₒ spec) α) : ProbComp (α × σ) :=
-  let so := (idOracle ++ₛₒ impl.baseSimOracle).maskState <| Equiv.punitProd σ
-  simulate so impl.init_state oa
+variable {ι : Type} {spec : OracleSpec ι} {σ α β γ : Type}
 
-def OracleImpl.exec' {ι : Type} {spec : OracleSpec ι} {α σ : Type}
-    (impl : OracleImpl spec σ) (oa : OracleComp (unifSpec ++ₒ spec) α) : ProbComp α :=
+/-- Run a computation `oa` using a given implementation `impl` of its oracles,
+with initial state `s`. Returns both the result and final state.
+The computation `oa` is assumed to also have access to uniform selection oracles,
+which are simulated by directly forwarding their calls with `idOracle`. -/
+def OracleImpl.run (impl : OracleImpl spec σ)
+    (oa : OracleComp (unifSpec ++ₒ spec) α) (s : σ) : ProbComp (α × σ) :=
   let so := (idOracle ++ₛₒ impl.baseSimOracle).maskState <| Equiv.punitProd σ
-  simulate' so impl.init_state oa
+  simulate so s oa
+
+/-- Shorthand for running a computation using the given oracle implementation,
+using the initial simulation state specified by the implementation itself. -/
+abbrev OracleImpl.exec (impl : OracleImpl spec σ)
+    (oa : OracleComp (unifSpec ++ₒ spec) α) : ProbComp (α × σ) :=
+  OracleImpl.run impl oa impl.init_state
+
+-- def OracleImpl.exec' (impl : OracleImpl spec σ)
+--     (oa : OracleComp (unifSpec ++ₒ spec) α) : ProbComp α :=
+--   let so := (idOracle ++ₛₒ impl.baseSimOracle).maskState <| Equiv.punitProd σ
+--   simulate' so impl.init_state oa
 
 namespace OracleImpl
+
+@[simp]
+lemma exec_pure (impl : OracleImpl spec σ) (x : α) (s : σ) :
+    impl.run (return x) s = return (x, s) := rfl
+
+@[simp]
+lemma exec_bind (impl : OracleImpl spec σ) (oa : OracleComp (unifSpec ++ₒ spec) α)
+    (ob : α → OracleComp (unifSpec ++ₒ spec) β) (s : σ) :
+    (impl.run (oa >>= ob) s = do let (x, s') ← impl.run oa s; impl.run (ob x) s') := by
+  simp [OracleImpl.run]
+
+-- @[simp]
+-- lemma exec_query (impl : OracleImpl spec σ) (i : ℕ ⊕ ι) (t : (unifSpec ++ₒ spec).domain i)
+--     (s : σ) : impl.run (query i t) s = sorry := sorry
 
 def emptyImpl : OracleImpl []ₒ Unit where
   baseSimOracle := unifOracle
